\mtexe{1.11}
\begin{proof}
    Exactly as before: for $\alpha,\beta \in \ZZ[\omega]$, we have
    \[ N(\alpha\beta) = (\alpha\beta)\overline{(\alpha\beta)} = \alpha\beta\overline{\alpha}\overline{\beta} = (\alpha\overline{\alpha})(\beta\overline{\beta}) = N(\alpha)N(\beta) \]
    So, if $\alpha \mid \gamma$ in $\ZZ[\omega]$, then there is $\beta \in \ZZ[\omega]$ with $\gamma = \alpha\beta$ and then $N(\gamma) = N(\alpha)N(\beta)$. Each of these norms is in $\ZZ$, so we have $N(\alpha) \mid N(\gamma)$.
\end{proof}