\mtexe{6.1.1}
\begin{proof}
	First, note that $d$ is $A$-linear, for if $a \in A$ and $b,b' \in B$, then
	\begin{align*}
		d(ab) &= (ab) \otimes 1 - 1 \otimes (ab) = a(b \otimes 1 - 1 \otimes b) = adb \\
		d(b+b') &= (b+b') \otimes 1 - 1 \otimes (b+b') = (b \otimes 1 - 1 \otimes b)+(b' \otimes 1 - 1 \otimes b') = db+db'
	\end{align*}
	Further, it satisfies the product rule:
	\[ d(bb')-bdb'-b'db = (bb') \otimes 1 - 1 \otimes (bb') - b(b' \otimes 1 - 1 \otimes b') - b'(b \otimes 1 - 1 \otimes b) = (bb') \otimes 1 - 1 \otimes (bb') - b' \otimes b - 1 \otimes (bb') - b \otimes b' - 1 \otimes (bb') = 
\end{proof}
